a lot of changes, no much progress

src/Infer.v
@@ -7,11 +7,13 @@ Require Import ListIds.
 Require Import Schemes.
 Require Import Rename.
 Require Import Disjoints.
+Require Import Program.
 Require Import Unify.
 Require Import Gen.
 Require Import Arith.Arith_base.
 Require Import Typing.
 Require Import List.
+Require Import NewTypeVariable.
 
 (** * State monad creator *)
 
@@ -21,7 +23,7 @@ Record tc_state := mkState {next_tvar : id}.
 
 Definition Infer (A : Type) := tc_state -> option (tc_state * A)%type.
 
-Definition ret (A : Type) (x : A) : Infer A := fun s => Some (s,x).
+Definition ret {A : Type} (x : A) : Infer A := fun s => Some (s,x).
 
 Definition failT (A : Type) : Infer A := fun s => None.
 
@@ -31,6 +33,14 @@ Definition bind (A B : Type) (c : Infer A) (c' : A -> Infer B) : Infer B :=
     | None => None
     | Some (s',v) => c' v s'            
     end.
+
+Lemma mon_left_id : forall (A B : Type) (a : A) (f : A -> Infer B), bind (ret a) f = f a.
+  intros.
+  reflexivity.
+Qed.
+
+Lemma mon_right_id : forall (A : Type) (a : Infer A), (bind a ret) = a.
+Admitted.
 
 Notation "x <- c1 ; c2" := (bind c1 (fun x => c2)) 
                             (right associativity, at level 84, c1 at next level).
@@ -46,9 +56,9 @@ Fixpoint mapM (A B : Type) (f : A -> Infer B) (l : list A) : Infer (list B) :=
   end.              
 
 (** Gives you a fresh variable *)
-Definition fresh : Infer ty :=
+Definition fresh : Infer id :=
   fun s => match s with
-          mkState n=> Some (mkState (1 + n), var n)
+          mkState n=> Some (mkState (1 + n), n)
         end.
 
 (** Gives a list of bound ids *)
@@ -59,26 +69,117 @@ Fixpoint list_bounds_ids_aux (sigma : schm) (g : list id) : list id :=
   | _ => nil
   end.
 
+Fixpoint max_gen_vars (sigma : schm) : nat :=
+  match sigma with
+  | sc_con _ => 0
+  | sc_var _ => 0
+  | sc_gen i => S i
+  | sc_arrow s1 s2 => max (max_gen_vars s1) (max_gen_vars s2)
+  end.
+
+Fixpoint compute_generic_subst (st : id) (n : nat): inst_subst * id :=
+  match n with
+  | O => (nil, st)
+  | S p =>
+      match compute_generic_subst (S st) p with
+      | (l, st') => (var st :: l, st')
+      end
+  end.
+
 Definition list_bounds_ids (sigma :schm) := list_bounds_ids_aux sigma nil.
 
+Fixpoint compute_subst (i : id) (l : list ty) : substitution :=
+  match l return substitution with
+  | nil => nil
+  | t :: l' => (i, t) :: compute_subst (S i) l'
+  end.
+
+
+(*
+    apply_inst_subst i_s sigma = Some_schm tau ->
+    apply_inst_subst i_s' (apply_subst_schm phi sigma) = Some_schm tau' ->
+    tau' = apply_subst ((compute_subst st i_s') ++ phi) tau.
+*)
+
+Lemma comute_inst_subst_subst : forall i_s s sigma tau tau', are_disjoints (ids_inst_subst i_s) (dom s) -> 
+    apply_inst_subst i_s (apply_subst_schm s sigma) = Some_schm tau ->
+    apply_inst_subst i_s sigma = Some_schm tau' ->
+    apply_subst s tau' = tau.
+Proof.
+  intros.
+  pose proof (subst_schm_when_dom_s_disjoint_with_FV_schm s sigma H) as K.
+Admitted.
+
+Definition compute_gen_subst2 (sigma : schm) :
+  Infer ({i_s : list ty & {s : list id | forall sigma i_s' tau phi, (
+                                                       are_disjoints s (FV_schm sigma) ->
+                                                       dom phi = s -> img phi = i_s' ->
+                                                       apply_inst_subst i_s sigma = Some_schm tau ->
+                                                       apply_inst_subst i_s' sigma = Some_schm (apply_subst phi tau))}}).
+  intros.
+  refine (match list_bounds_ids sigma with
+  | lv =>
+        s <- mapM (fun _ => fresh) lv ;
+        match (map (fun i => (var i)) s) with
+        | i_s =>  ret (existT _ i_s (exist _ s _))
+        end 
+  end) . 
+  intros.
+  assert (i_s = map (fun i : id => var i) s ) as Y.
+  { reflexivity. }
+  rewrite <- H0 in H.
+  pose proof (subst_schm_when_dom_s_disjoint_with_FV_schm phi sigma0 H) as K.
+  unfold are_disjoints in H.
+  induction i_s.
+  - cases s.
+    simpl in H.
+    symmetry in H.
+    rewrite length_zero_iff_nil in H.
+    subst.
+    simpl.
+    auto.
+    symmetry in H.
+    rewrite length_zero_iff_nil in H.
+    subst.
+    simpl.
+    auto.
+  - apply IHi_s; auto.
+  destruct i_s.
+  skip.
+Defined.
+
 (** Gives a type that is a (new) instance of a scheme *)
-Definition schm_inst_dep : forall (sigma : schm), Infer ({tau : ty | is_schm_instance tau sigma}).
-  refine(fix schm_inst_dep (sigma : schm) :
-           Infer ({tau : ty | is_schm_instance tau sigma}) :=
-           match list_bounds_ids sigma  with
-           | lv =>
-             s <- mapM (fun _ => fresh) lv ;
-             match apply_inst_subst s sigma as y' return
-                   apply_inst_subst s sigma = y' ->
-                   Infer ({tau : ty | is_schm_instance tau sigma}) with
-             | Error_schm => fun H0 => (failT _) 
-             | Some_schm tau => fun H => (ret (exist _ tau _))
-             end _
-           end).
-  unfold is_schm_instance.
-  exists s.
-  auto.
-  auto.
+Definition schm_inst_dep : forall (sigma : schm),
+    Infer ({tau | exists i_s, apply_inst_subst i_s sigma = (Some_schm tau) /\
+           (forall tau' i_s' phi, apply_inst_subst i_s' (apply_subst_schm phi sigma) = Some_schm tau' ->
+                             exists s, tau' = apply_subst (s ++ phi) tau )}).
+  intros.
+  refine(
+          match compute_gen_subst2 sigma as y return compute_gen_subst2 sigma = y -> _ with
+          | r => fun H1 => 
+               i_ss <- r ;
+               match i_ss with | existT _ i_s0 (exist _ s0 _) =>
+               match apply_inst_subst i_s0 sigma as y' return apply_inst_subst i_s0 sigma = y' -> _ with
+               | Error_schm => fun H0 => (failT _) 
+               | Some_schm tau => fun H => (ret (exist _ tau _))
+               end _  end
+           end _).
+  exists i_s0.
+  split.
+  - auto.
+  - intros.
+    destruct a with (i_s' := i_s') (sigma := sigma) (tau:=tau).
+    clear H1 r i_ss s a.
+    sort.
+    apply H3 in H as H'.
+    exists (combine s0 i_s').
+    rewrite apply_subst_append.
+    symmetry.
+    eapply comute_inst_subst_subst.
+    apply H0.
+    auto.
+  - reflexivity.
+  - reflexivity.
 Defined.
 
 Definition  look_dep : forall (x : id) (G : ctx), Infer {sigma | in_ctx x G = Some sigma}.
@@ -108,10 +209,68 @@ Definition  look_const_dep : forall (x : id) (G : ctx), Infer {sigma & {i | in_c
   mysimp.
 Qed.
 
+
+Definition getResult (A B : Type) {P} (rs : option (tc_state * (({ti : A & {s : B | P ti s}}))))
+  : option (id * A * B) :=
+  match rs with
+  | None => None
+  | Some (mkState i, (existT _ t (exist _ s P))) => Some (i, t ,s)
+  end.
+
+Definition getInst (A : Type) {P} (rs : option (tc_state * {x : A | P x}))
+  : option A :=
+  match rs with
+  | None => None
+  | Some (mkState i, exist _ s _) => Some s
+  end.
+
+Lemma assoc_subst_exists : forall (G : ctx) (i : id) (s : substitution) (sigma : schm),
+    in_ctx i (apply_subst_ctx s G) = Some sigma ->
+    {sigma' : schm | in_ctx i G = Some sigma' /\ sigma = apply_subst_schm s sigma'}.
+Proof.
+Admitted.
+
+Definition completeness (e : term) (G : ctx) (tau : ty) (s : substitution) :=
+  forall (tau' : ty) (phi : substitution) (st : id),
+    has_type (apply_subst_ctx phi G) e tau' -> new_tv_ctx G st ->
+    exists s', tau' = apply_subst s' tau /\
+    (forall x : id, x < st -> apply_subst phi (var x) = apply_subst (s ++ s') (var x)).
+
+Lemma t_is_app_T_aux : forall (sigma : schm) (tau tau' : ty) (s : substitution) (p : nat) (st : id) (x : list ty),
+    new_tv_schm sigma st -> max_gen_vars sigma <= p ->
+    apply_inst_subst (fst (compute_generic_subst st p)) sigma = Some_schm tau ->
+    apply_inst_subst x (apply_subst_schm s sigma) = Some_schm tau' ->
+    tau' = apply_subst ((compute_subst st x) ++ s) tau.
+Proof.
+  Admitted.
+
+Lemma t_is_app_T_aux' : forall (sigma : schm) (tau tau' : ty) (phi : substitution) (p : nat) (st : id) (i_s i_s' : list ty),
+    new_tv_schm sigma st -> max_gen_vars sigma <= p ->
+    apply_inst_subst i_s sigma = Some_schm tau ->
+    apply_inst_subst i_s' (apply_subst_schm phi sigma) = Some_schm tau' ->
+    tau' = apply_subst ((compute_subst st i_s') ++ phi) tau.
+Proof.
+  Admitted.
+
+Lemma new_tv_ctx_implies_new_tv_schm : forall (G : ctx) (sigma : schm) (st x : id),
+    in_ctx x G = Some sigma -> new_tv_ctx G st -> new_tv_schm sigma st.
+Proof.
+  Admitted.
+
+Lemma list_ty_and_id_inv : forall lt_st : list ty * id,
+    {lt_st1 : list ty * id | lt_st1 = lt_st}.
+Proof.
+intros lt_st; exists lt_st; auto.
+Qed.
+
+Lemma apply_compute_gen_subst : forall (i : id) (sigma : schm) (p : nat) i_s,
+    {tau : ty | apply_inst_subst i_s sigma = Some_schm tau}.
+Admitted.
+
 Definition infer_dep : forall (e : term) (G : ctx),
-    Infer ({tau : ty & {s : substitution | has_type (apply_subst_ctx s G) e tau}}).
+    Infer ({tau : ty & {s : substitution | has_type (apply_subst_ctx s G) e tau /\ completeness e G tau s}}).
   refine (fix infer_dep (e : term) (G : ctx) :
-            Infer ({tau : ty & {s : substitution | has_type (apply_subst_ctx s G) e tau}}) :=
+            Infer ({tau : ty & {s : substitution | has_type (apply_subst_ctx s G) e tau /\ completeness e G tau s}}) :=
             match e with
             | const_t x =>
               sigma_dep <- look_dep x G ;
@@ -133,10 +292,10 @@ Definition infer_dep : forall (e : term) (G : ctx),
               end
             | lam_t x e =>
               alpha <- fresh ;
-              taus <- infer_dep e ((x, ty_to_schm alpha) :: G) ;
+              taus <- infer_dep e ((x, ty_to_schm (var alpha)) :: G) ;
               match taus with
               | (existT _ tau (exist _ s' p)) =>
-                ret (existT _ ( (arrow (apply_subst s' alpha) tau)) (exist _ s' _))
+                ret (existT _ ( (arrow (apply_subst s' (var alpha)) tau)) (exist _ s' _))
               end 
             | app_t l rho =>
               taus <- infer_dep l G ;
@@ -146,8 +305,8 @@ Definition infer_dep : forall (e : term) (G : ctx),
                 match taus' with
                 | existT _ tau' (exist _ s' p') => 
                   alpha <- fresh ;
-                  match unify_simple_dep (apply_subst s' tau) (arrow tau' alpha) with
-                  | existT _ c (inleft _ (exist _ x HS)) => ret (existT _ (apply_subst x alpha) (exist _ (s ++ s' ++ x) _))
+                  match unify_simple_dep (apply_subst s' tau) (arrow tau' (var alpha)) with
+                  | existT _ c (inleft _ (exist _ x HS)) => ret (existT _ (apply_subst x (var alpha)) (exist _ (s ++ s' ++ x) _))
                   | existT _ c _ => failT _
                   end
                 end
@@ -166,11 +325,147 @@ Definition infer_dep : forall (e : term) (G : ctx),
                 
             end).
   - clear infer_dep.
-    eapply var_ht.
-    rewrite apply_subst_ctx_nil.
-    apply pS.
-    apply A.
+    assert (has_type (apply_subst_ctx [] G) (var_t x) tau) as HST1.
+    { eapply var_ht. rewrite apply_subst_ctx_nil. apply pS. destruct A.  destruct H. unfold is_schm_instance. exists x0. apply H. }
+    split.
+    + apply HST1.
+    + unfold completeness.
+      intros.
+      clear etau sigma_dep.
+      rename H into HST2.
+      rename A into i_s_is_tau_and_compute_gen.
+      sort.
+      destruct i_s_is_tau_and_compute_gen as [i_s i_s_tau_compute_gen].
+      destruct i_s_tau_compute_gen.
+      destruct H.
+      inversion HST2.
+      destruct (assoc_subst_exists G x phi H2) as [sigma'  Hi].
+      destruct Hi.
+      rewrite H6 in pS.
+      inversion pS.
+      subst.
+      destruct H4.
+      apply H1 in H.
+      destruct H.
+      exists (x1 ++ phi).
+      split.
+      * auto.
+      *
+
+
+
+        destruct H3 as [i_s'].
+      exists (compute_subst st i_s' ++ phi).
+      rewrite inCtx in pS.
+      inversion pS.
+      subst.
+      split.
+      *
+        eapply t_is_app_T_aux.
+        eapply new_tv_ctx_implies_new_tv_schm. 
+        apply inCtx. auto.
+        skip.
+        auto.
+      exists (i_s ++ phi).
+      split.
+      * eapply H1.
+        subst.
+        
+        skip.
+        skip.
+        (* parei aqui *)
+        simpl.
+
+        
+      
+      rewrite apply_subst_ctx_nil in HST1.
+      apply has_type_is_stable_under_substitution with (s:=phi) in HST1 as HST3.
+      inversion HST2.
+      inversion HST3.
+      destruct H3.
+      subst. sort.
+      destruct A as [i_s].
+        destruct (list_ty_and_id_inv (compute_generic_subst st (max_gen_vars sigma))) as [GEN GENC].
+        destruct A.
+        destruct (apply_compute_gen_subst st sigma (max_gen_vars sigma) x0).
+        rewrite e0 in H.
+        inversion H.
+        subst.
+        eapply t_is_app_T_aux.
+        eapply new_tv_ctx_implies_new_tv_schm. 
+        apply pS; auto.
+        auto.
+        skip.
+        destruct A.
+        skip.
+        skip.
+      * appl
+
+
+        
+      clear etau.
+      destruct A.
+      sort.
+      inversion HST1.
+      inversion HST2.
+      inversion HST3.
+      subst.
+      destruct (assoc_subst_exists G x phi H12) as [sigma''  Hi'].
+      destruct Hi.
+      destruct Hi'.
+      sort.
+      rewrite H5 in H.
+      inversion H.
+      rewrite H10 in H6.
+      rewrite <- H6 in H3.
+      subst. sort.
+      
+      subst.
+      rewrite H1 in pS.
+      inversion pS.
+      subst.
+      sort.
+      inversion HST in H.
+      subst.
+      destruct (assoc_subst_exists G x phi H2) as [sigma''  Hi'].
+      destruct Hi'.
+      inversion H7.
+      assert (sigma'' = sigma). skip.
+      subst.
+
+               
+      inve
+
+      
+      simpl in HST.
+      remember A as A'.
+      clear HeqA'.
+      sort.
+      subst.
+      exists phi.
+      simpl.
+      
+      exists ((compute_subst st i_s) ++ nil).
+      splits.
+      
+      in
+      subst.
+
+      
+      inversion H.
+      destruct H6.
+      destruct a.
+      substs.
+      rewrite pS in H6.
+      inversion H6.
+      substs. clear H6. sort.
+
+
+      pose proof (assoc_subst_exists G x phi H2).
+      inversion H6 in pS.
+      unfold is_schm_instance in H4.
   - clear infer_dep taus taus' s1 s0 s2 s3.
+    split.
     simpl in HS.
     destruct HS.
     destruct H.
@@ -186,7 +481,11 @@ Definition infer_dep : forall (e : term) (G : ctx),
     apply p.
     apply has_type_is_stable_under_substitution.
     apply p'.
+    skip.
   - clear infer_dep taus taus' s0 s1.
+    skip.
+    (**
+    destruct p'.
     pose proof exists_renaming_not_concerned_with2 (gen_ty_vars tau (apply_subst_ctx s G))
          (FV_ctx (apply_subst_ctx s G)) (FV_subst s')  as lol.
     destruct lol as [rho].
@@ -212,16 +511,21 @@ Definition infer_dep : forall (e : term) (G : ctx),
     rewrite <- subst_add_type_scheme.
     rewrite <- gen_alpha4_bis; auto.
     auto.
+    *)
   - clear infer_dep s taus.
+    split.
     simpl in p.
     rewrite ty_to_subst_schm in p.
     eapply lam_ht.
     apply p.
+    skip.
   - clear infer_dep.
+    split.
     econstructor.
     rewrite apply_subst_ctx_nil.
     apply pS.
     apply A.
+    skip.
 Defined.
 
 Definition runInfer_id e g i := infer_dep e g (mkState i).
@@ -229,16 +533,3 @@ Definition runInfer e g := infer_dep e g (mkState 0).
 
 Compute runInfer (var_t 0) nil.
 
-Definition getResult (A B : Type) {P} (rs : option (tc_state * (({ti : A & {s : B | P ti s}}))))
-  : option (id * A * B) :=
-  match rs with
-  | None => None
-  | Some (mkState i, (existT _ t (exist _ s P))) => Some (i, t ,s)
-  end.
-
-Definition getInst (A : Type) {P} (rs : option (tc_state * {x : A | P x}))
-  : option A :=
-  match rs with
-  | None => None
-  | Some (mkState i, exist _ s _) => Some s
-  end.
